Flesh out some helper functions to the point where we can write down the preconditions and most of the post conditions. Still need to figure out the mapping from qb' to db'

ironfleet/src/Dafny/Distributed/Concur/QuantizedSystem.s.dfy
@@ -1,9 +1,13 @@
 include "../Common/Framework/Host.s.dfy"
+include "../Common/Framework/DistributedSystem.s.dfy"
 include "../Common/Collections/Maps2.s.dfy"
+include "../Common/Collections/Seqs.i.dfy"
 
 abstract module QuantizedSystem_s {
     import opened Host_s
     import opened Collections__Maps2_s
+    import opened DistributedSystem_s
+    import opened Collections__Seqs_i
 
     /////////////////////////////////////////
     // PHYSICAL ENVIRONMENT
@@ -55,6 +59,8 @@ abstract module QuantizedSystem_s {
         && LEnvironment_Init(s.environment)
         && (forall id :: id in s.servers ==> HostInit(s.servers[id], config, id))
     }
+
+    predicate QuantizedHostNext(s:HostState, s':HostState, ios:seq<LIoOp<EndPoint,seq<byte>>>)
     
     predicate QS_NextOneServer(s:QS_State, s':QS_State, id:EndPoint, ios:seq<LIoOp<EndPoint,seq<byte>>>)
         requires id in s.servers;
@@ -78,22 +84,72 @@ abstract module QuantizedSystem_s {
                s'.servers == s.servers
     }
 
-    lemma BryansProof(config:ConcreteConfiguration, qb:seq<QS_State>, P:Predicate) returns (qb':seq<QS_State, db':seq<DS_State>, cm:seq<int>)
+    type StepTrace = seq<LEnvStep<EndPoint,seq<byte>>>
+    type IoOp = LIoOp<EndPoint,seq<byte>>
+    type IoTrace = seq<IoOp>
+
+    function {:opaque} ComputeStepTrace(qb:seq<QS_State>) : StepTrace
+        ensures |qb| == |ComputeStepTrace(qb)|;                                               
+        ensures forall i :: 0 <= i < |qb| ==> ComputeStepTrace(qb)[i] == qb[i].environment.nextStep;
+    {
+        if qb == [] then
+            []
+        else
+            [qb[0].environment.nextStep] + ComputeStepTrace(qb[1..])
+    }
+
+    function ProjectStepTraceToHostIos(trace:StepTrace, host:EndPoint) : IoTrace
+    {
+        if trace == [] then
+            []
+        else
+            if trace[0].LEnvStepHostIos? && trace[0].actor == host then
+                trace[0].ios + ProjectStepTraceToHostIos(trace[1..], host)
+            else
+                ProjectStepTraceToHostIos(trace[1..], host)
+    }
+
+    function ProjectExternalIO(qb:seq<QS_State>, config:ConcreteConfiguration, external_io:(IoOp, ConcreteConfiguration) -> bool) : IoTrace
+        requires forall io :: external_io.requires(io, config);
+        reads    external_io.reads;
+    {
+        if qb == [] then 
+            []
+        else
+            var step := qb[0].environment.nextStep;
+            if step.LEnvStepHostIos? && |step.ios| == 1 && external_io(step.ios[0], config) then
+                step.ios + ProjectExternalIO(qb[1..], config, external_io)
+            else
+                ProjectExternalIO(qb[1..], config, external_io)
+    }
+
+    lemma BryansProof(config:ConcreteConfiguration, qb:seq<QS_State>, external_io:(IoOp, ConcreteConfiguration) -> bool) returns (qb':seq<QS_State>, db':seq<DS_State>, cm:seq<int>)
         requires |qb| > 0;
         requires QS_Init(qb[0], config);
         requires forall i {:trigger QS_Next(qb[i], qb[i+1])} :: 0 <= i < |qb| - 1 ==> QS_Next(qb[i], qb[i+1]);
                 
-        requires 
-                 var trace:seq<IO> := ComputeTrace(qb);
-            forall host :: host in .servers ==> exists io_partition:seq<seq<IO>>, behavior:seq<DS_State> :: SeqCat(io_partition) == Restrict(trace, host) && |io_partition| == | behavior| && forall i :: 0 <= i < |io_partition| ==> HostNext(behavior[i], behavior[i+1], io_partition[i]);
+        requires var trace:StepTrace := ComputeStepTrace(qb);
+                 forall host :: host in qb[0].servers ==> 
+                     exists io_partition:seq<IoTrace>, behavior:seq<HostState> :: 
+                         SeqCat(io_partition) == ProjectStepTraceToHostIos(trace, host) 
+                      && |io_partition| == |behavior| - 1
+                      && (forall i :: 0 <= i < |io_partition| ==> HostNext(behavior[i], behavior[i+1], io_partition[i]));
+        ensures  |qb| == |qb'|;
+        ensures  QS_Init(qb'[0], config);
+        ensures  forall i {:trigger QS_Next(qb'[i], qb'[i+1])} :: 0 <= i < |qb'| - 1 ==> QS_Next(qb'[i], qb'[i+1]);
+        ensures  ProjectExternalIO(qb, config, external_io) == ProjectExternalIO(qb', config, external_io);
 
-        ensures  |qb| == |cm|;
-        ensures  cm[0] == 0;                                            // Beginnings match
+        ensures  |qb'| == |cm|;
+        ensures  cm[0] == 0;                                             // Beginnings match
         ensures  forall i :: 0 <= i < |cm| ==> 0 <= cm[i] < |db'|;       // Mappings are in bounds
         ensures  forall i {:trigger cm[i], cm[i+1]} :: 0 <= i < |cm| - 1 ==> cm[i] <= cm[i+1];    // Mapping is monotonic
         ensures  DB_Init(db'[0], config);
         ensures  forall i {:trigger DS_Next(db'[i], db'[i+1])} :: 0 <= i < |db'| - 1 ==> DS_Next(db'[i], db'[i+1]);
 
+        // TODO: Need to relate qb' and db'
+
+
+/*
         ensures  forall i :: 0 <= i < |qb| ==> Correspondence(qb[i].environment.sentPackets, db'[cm[i]]);
 
         ensures forall i :: 0 <= i < |qb'| ==> 
@@ -110,5 +166,6 @@ abstract module QuantizedSystem_s {
                     )
         ensures forall packets, packets' :: packets <= packets' ==> (P(packets) ==> P(packets'))        # Probably not true
         ensures forall packets, packets' :: packets <= packets' ==> (P(packets) <== P(packets'))
+*/
 }
 
